theories/typing/adequacy.v
@@ -9,12 +9,14 @@ Set Default Proof Using "Type".
 Class typePreG Σ := PreTypeG {
   type_invG :> invPreG Σ;
   type_heap_inG :> inG Σ (authR heapUR);
+  type_heap_allocs_inG :> inG Σ (authR allocsUR);
   type_heap_fntbl_inG :> inG Σ (authR fntblUR);
 }.
 
 Definition typeΣ : gFunctors :=
   #[invΣ;
     GFunctor (constRF (authR heapUR));
+    GFunctor (constRF (authR allocsUR));
     GFunctor (constRF (authR fntblUR))].
 Instance subG_typePreG {Σ} : subG typeΣ Σ → typePreG Σ.
 Proof. solve_inG. Qed.
@@ -30,10 +32,10 @@ Definition initial_thread_state (main : loc) : thread_state := {|
   ts_conts := [];
 |}.
 
-Definition initial_state (fns : gmap loc function) (gs : gmap loc mbyte) :=
+Definition initial_state (fns : gmap loc function) (gs : gmap loc mbyte) (bs : blocks) :=
   {| st_heap := (λ b, (RSt 0%nat, b) ) <$> gs;
      st_fntbl := fns;
-     st_used_blocks := list_to_set (map_to_list gs).*1.*1 |}.
+     st_used_blocks := bs |}.
 
 Lemma wp_to_typed_stmt `{!typeG Σ} (ts : thread_state) v':
   f_code (rf_fn (ts_rfn ts)) = ∅ →
@@ -48,49 +50,63 @@ Proof.
 Qed.
 
 Definition main_type `{!typeG Σ} (P : iProp Σ) :=
-    fn(∀ () : (); P) → ∃ () : (), int i32; True.
+  fn(∀ () : (); P) → ∃ () : (), int i32; True.
 
 (** * The main adequacy lemma *)
-Lemma refinedc_adequacy Σ `{!typePreG Σ} (thread_mains : list loc) (fns : gmap loc function) (gs : gmap loc mbyte) n t2 σ2 κs:
+Lemma refinedc_adequacy Σ `{!typePreG Σ} (thread_mains : list loc) (fns : gmap loc function) (gs : gmap loc mbyte) (bs : blocks) n t2 σ2 κs:
+  blocks_used_agree (initial_state fns gs bs).(st_heap) (initial_state fns gs bs).(st_used_blocks) →
   (∀ {HtypeG : typeG Σ}, ∃ gl gt,
   let Hglobals : globalG Σ := {| global_locs := gl; global_initialized_types := gt; |} in
-      ([∗ map] k↦qs∈gs, k ↦ [qs]) -∗ ([∗ map] k↦qs∈fns, fntbl_entry k qs) ={⊤}=∗
+    ([∗ map] k↦qs∈gs, heap_mapsto_mbyte k 1 qs) -∗
+    ([∗ map] k↦qs∈bs, allocs_entry k qs) -∗
+    ([∗ map] k↦qs∈fns, fntbl_entry k qs) ={⊤}=∗
       [∗ list] main ∈ thread_mains, ∃ P, main ◁ᵥ main @ function_ptr (main_type P) ∗ P) →
-  nsteps (Λ := stmt_lang) n (initial_thread_state <$> thread_mains, initial_state fns gs ) κs (t2, σ2) →
+  nsteps (Λ := stmt_lang) n (initial_thread_state <$> thread_mains, initial_state fns gs bs) κs (t2, σ2) →
   ∀ e2, e2 ∈ t2 → not_stuck e2 σ2.
 Proof.
-  move => Hwp. apply: wp_strong_adequacy. move => ?.
+  move => Hvalid Hwp. apply: wp_strong_adequacy. move => ?.
   set h := to_heap ((λ b, (RSt 0%nat, b)) <$> gs).
   iMod (own_alloc (● h ⋅ ◯ h)) as (γh) "[Hh Hm]" => //.
   { apply auth_both_valid_discrete. split => //. eauto using to_heap_valid. }
   set f := to_fntbl fns.
   iMod (own_alloc (● f ⋅ ◯ f)) as (γf) "[Hf Hfm]" => //.
   { apply auth_both_valid_discrete. split => //. eauto using to_fntbl_valid. }
+  set b := to_allocs bs.
+  iMod (own_alloc (● b ⋅ ◯ b)) as (γb) "[Hb #Hbm]" => //.
+  { apply auth_both_valid_discrete. split => //. eauto using to_allocs_valid. }
 
-  set (HheapG := HeapG _ _ γh _ γf).
+  set (HheapG := HeapG _ _ γh _ γb _ γf).
   set (HrefinedCG := RefinedCG _ _ HheapG).
   set (HtypeG := TypeG _ HrefinedCG).
   move: (Hwp HtypeG) => {Hwp} [gl [gt]].
   set (Hglobals := {| global_locs := gl; global_initialized_types := gt; |}).
   move => Hwp.
-  iMod (Hwp with "[Hm] [Hfm]") as "Hmains". {
-    rewrite /h => {h Hwp}.
-    iInduction (gs) as [|?????] "IH" using map_ind => //.
-    iApply big_sepM_insert => //. rewrite fmap_insert to_heap_insert.
-    rewrite (insert_singleton_op). 2: by apply lookup_to_heap_None; simplify_map_eq.
-    iDestruct "Hm" as "[Hx Hm]". rewrite heap_mapsto_cons heap_mapsto_nil heap_mapsto_mbyte_eq. iFrame.
+  iMod (Hwp with "[Hm] [] [Hfm]") as "Hmains". {
+    rewrite /h => {h Hwp Hvalid}.
+    iInduction (gs) as [|i ????] "IH" using map_ind => //.
+    iApply big_sepM_insert => //.
+    rewrite fmap_insert to_heap_insert insert_singleton_op. 2: by apply lookup_to_heap_None; simplify_map_eq.
+    rewrite heap_mapsto_mbyte_eq /heap_mapsto_mbyte_def /=.
+    iDestruct "Hm" as "[$ Hm]".
     by iApply "IH".
   } {
-    rewrite /f => {f Hwp}.
+    rewrite /b => {b Hwp Hvalid}.
+    iInduction (bs) as [|??? HNone] "IH" using map_ind => //.
+    iApply big_sepM_insert => //. rewrite /to_allocs fmap_insert.
+    rewrite (insert_singleton_op); last by rewrite lookup_fmap HNone.
+    rewrite allocs_entry_eq. iDestruct "Hbm" as "[$ Hfm]".
+    by iApply "IH".
+  } {
+    rewrite /f => {f Hwp Hvalid}.
     iInduction (fns) as [] "IH" using map_ind => //.
     iApply big_sepM_insert => //. rewrite to_fntbl_insert.
     rewrite (insert_singleton_op); last by apply lookup_to_fntbl_None.
-    iDestruct "Hfm" as "[Hx Hfm]". rewrite fntbl_entry_eq. iFrame.
+    rewrite fntbl_entry_eq. iDestruct "Hfm" as "[$ Hfm]".
     by iApply "IH".
   }
 
   iModIntro. iExists NotStuck, _, (replicate (length thread_mains) (λ _, True%I)), _.
-  iSplitL "Hh Hf"; last first. 1: iSplitL.
+  iSplitL "Hh Hb Hf"; last first. 1: iSplitL.
   - rewrite big_sepL2_fmap_l. iApply big_sepL2_replicate_2. iApply (big_sepL_impl with "Hmains").
     iIntros "!#" (? main ?); iDestruct 1 as (P) "[Hmain HP]".
     iApply wp_to_typed_stmt => //.
@@ -100,16 +116,13 @@ Proof.
     simpl_subst. iApply type_return. iApply type_val. iApply type_void.
     iIntros (_). by iExists ().
   - iFrame. iIntros (?? _ _ ?) "_ _ _". iApply fupd_mask_weaken => //. iPureIntro. by eauto.
-  - iFrame. iPureIntro => /=. clear. move => l Hl i. rewrite lookup_fmap fmap_None.
-    destruct (gs !! (l +ₗ i)) as [x|] eqn:? => //. exfalso. apply: Hl.
-    apply elem_of_list_to_set. apply elem_of_list_fmap. exists (l +ₗ i). split. by destruct l.
-    apply elem_of_list_fmap. eexists (_, x). split => //. apply elem_of_map_to_list. by destruct l.
+  - by iFrame.
 Qed.
 
 (** * Helper functions for using the adequacy lemma *)
-Definition block_to_loc (l: Z): loc := (l, 0%Z).
+Definition block_to_loc (l: block_id): loc := (l, 0%Z).
 
-Definition block_list_to_loc (l: Z): list mbyte → gmap loc mbyte :=
+Definition block_list_to_loc (l: block_id): list mbyte → gmap loc mbyte :=
   list_to_map ∘ imap (λ i b, (block_to_loc l +ₗ i, b)).
 
 Lemma block_list_to_loc_nil l :
@@ -136,29 +149,53 @@ Proof.
   apply not_elem_of_list_to_map_1 => /= Hin2. set_solver.
 Qed.
 
-Definition heap_list_to_heap : gmap Z (list mbyte) → gmap loc mbyte :=
+Definition heap_list_to_heap : gmap block_id (list mbyte) → gmap loc mbyte :=
   map_fold (λ b ls m, block_list_to_loc b ls ∪ m) ∅.
+
+Definition heap_list_to_used_blocks : gmap block_id (list mbyte) → blocks :=
+    fmap (λ l, to_allocation 0 (length l)).
 
 Lemma heap_list_to_heap_insert `{!refinedcG Σ} l v h :
   h !! l = None →
-  ([∗ map] k↦qs ∈ heap_list_to_heap (<[l := v]> h), k ↦ [qs]) -∗
-  block_to_loc l ↦ v ∗ ([∗ map] k↦qs ∈ heap_list_to_heap h, k ↦ [qs]).
+  ([∗ map] k↦qs ∈ heap_list_to_heap (<[l := v]> h), heap_mapsto_mbyte k 1 qs) -∗
+  ([∗ map] k↦qs ∈ heap_list_to_used_blocks (<[l := v]> h), allocs_entry k qs) -∗
+  block_to_loc l ↦ v ∗
+  ([∗ map] k↦qs ∈ heap_list_to_heap h, heap_mapsto_mbyte k 1 qs) ∗
+  ([∗ map] k↦qs ∈ heap_list_to_used_blocks h, allocs_entry k qs).
 Proof.
-  iIntros (HNone) "Hm".
+  iIntros (HNone) "Hm Ha".
   rewrite /heap_list_to_heap map_fold_insert_L //; last by move => *; apply block_list_to_loc_comm.
-  rewrite big_sepM_union.
-  - iDestruct "Hm" as "[Hv $]".
-    iInduction (v) as [] "IH" using rev_ind. by rewrite heap_mapsto_nil.
-    rewrite block_list_to_loc_app heap_mapsto_app big_sepM_insert.
-    + iDestruct "Hv" as "[$ Hl]". by iApply "IH".
-    + apply not_elem_of_list_to_map_1. set_unfold.
-      move => [[??][?[?[?[?/(lookup_lt_Some _ _ _) ?]]]]]. naive_solver lia.
-  - apply/map_disjoint_list_to_map_l/Forall_forall => *.
+  rewrite big_sepM_union. 2: {
+    apply/map_disjoint_list_to_map_l/Forall_forall => *.
     induction h using map_ind => //.
     move: HNone => /lookup_insert_None [??].
     rewrite map_fold_insert_L //; last by move => *; apply block_list_to_loc_comm.
     apply lookup_union_None. split; last by eauto.
     apply not_elem_of_list_to_map_1. set_solver.
+  }
+  iDestruct "Hm" as "[Hv $]".
+  rewrite /heap_list_to_used_blocks fmap_insert big_sepM_insert; last by rewrite lookup_fmap HNone.
+  iDestruct "Ha" as "[Ha $]".
+  rewrite heap_mapsto_eq/heap_mapsto_def.
+  iSplitL "Ha". { iApply allocs_entry_to_loc_in_bounds => //. simpl. lia. }
+  iInduction (v) as [] "IH" using rev_ind => //.
+  rewrite block_list_to_loc_app big_sepM_insert ?big_sepL_app /= ?Nat.add_0_r.
+  + iDestruct "Hv" as "[$ Hl]". by iApply "IH".
+  + apply not_elem_of_list_to_map_1. set_unfold.
+    move => [[??][?[?[?[?/(lookup_lt_Some _ _ _) ?]]]]]. naive_solver lia.
+Qed.
+
+Lemma heap_list_blocks_agree fns gs:
+  blocks_used_agree (initial_state fns (heap_list_to_heap gs) (heap_list_to_used_blocks gs)).(st_heap) (initial_state fns (heap_list_to_heap gs) (heap_list_to_used_blocks gs)).(st_used_blocks).
+Proof.
+  move => /= l. rewrite /heap_list_to_used_blocks lookup_fmap fmap_None. move => Hgs i.
+  rewrite lookup_fmap fmap_None /heap_list_to_heap. move: Hgs.
+  induction gs as [|] using map_ind. { by rewrite map_fold_empty. }
+  rewrite map_fold_insert_L //; last by move => *; apply block_list_to_loc_comm.
+  move => /lookup_insert_None[??]. apply/lookup_union_None. split; [ | naive_solver ].
+  rewrite /block_list_to_loc /= not_elem_of_list_to_map_1 //.
+  move => /elem_of_list_fmap[[??]/=[?]] /(elem_of_lookup_imap_1 _ _ _)[? [?[??]]].
+  simplify_eq.
 Qed.
 
 Definition fn_lists_to_fns (locs : list loc) (fns : list function) : gmap loc function :=
