theories/typing/padded.v
@@ -7,10 +7,12 @@ Section padded.
 
   Program Definition padded (ty : type) (lyty ly : layout) : type := {|
     ty_own β l :=
-      ⌜lyty ⊑ ly⌝ ∗ ⌜l `has_layout_loc` ly⌝ ∗ l ◁ₗ{β} ty ∗ (l +ₗ lyty.(ly_size)) ◁ₗ{β} uninit (ly_offset ly lyty.(ly_size));
+      ⌜lyty ⊑ ly⌝ ∗ ⌜l `has_layout_loc` ly⌝ ∗
+      loc_in_bounds l ly.(ly_size) ∗
+      l ◁ₗ{β} ty ∗ (l +ₗ lyty.(ly_size)) ◁ₗ{β} uninit (ly_offset ly lyty.(ly_size));
   |}%I.
   Next Obligation.
-    iDestruct 1 as "[$ [$ [HT Hl]]]".
+    iDestruct 1 as "[$ [$ [$ [HT Hl]]]]".
     iMod (ty_share with "HT") as "$" => //.
     by iApply ty_share.
   Qed.
@@ -32,7 +34,7 @@ Section padded.
     iPureIntro. rewrite /has_layout_val app_length Heq1 Heq2 Heq {2}/ly_size/=. lia.
   Qed.
   Next Obligation.
-    iIntros (ty lyty ly ? Heq l). iDestruct 1 as ([??] ?) "[Hl Hpad]".
+    iIntros (ty lyty ly ? Heq l). iDestruct 1 as ([??] ?) "[_ [Hl Hpad]]".
     iDestruct (ty_deref with "Hl") as (v1) "[Hmt1 Hv1]".
     iDestruct (ty_size_eq with "Hv1") as %Heq1.
     iDestruct (ty_deref with "Hpad") as (v2) "[Hmt2 Hv2]".
@@ -42,16 +44,25 @@ Section padded.
   Next Obligation.
     iIntros (ty lyty ly ? <- l v Hly) "Hmt". iDestruct 1 as (v1 v2 [??] ->) "[Hv1 Hv2]".
     iDestruct (ty_size_eq with "Hv1") as %Heq1.
+    iDestruct (ty_size_eq with "Hv2") as %Heq2.
+    iDestruct (heap_mapsto_loc_in_bounds with "Hmt") as "#Hb".
     rewrite heap_mapsto_app Heq1.
     iDestruct "Hmt" as "[Hmt1 Hmt2]".
     iDestruct (ty_ref with "[%] Hmt1 Hv1") as "$". by apply: has_layout_loc_trans.
     iDestruct (ty_ref with "[%] Hmt2 Hv2") as "$" => //. by apply: has_layout_ly_offset.
+    iSplit => //. iSplit => //. iApply loc_in_bounds_shorten; last done.
+    rewrite app_length Heq1 Heq2 /ly_size /= -!/(ly_size _). lia.
+  Qed.
+
+  Global Instance loc_in_bounds_padded ty lyty ly β: LocInBounds (padded ty lyty ly) β.
+  Proof.
+    constructor. iIntros (l) "(_&_&H&_)". iApply loc_in_bounds_shorten; last done. lia.
   Qed.
 
   Lemma simpl_padded_hyp_eq_layout l β ty ly T:
     (l ◁ₗ{β} ty -∗ T) -∗
     simplify_hyp (l ◁ₗ{β} padded ty ly ly) T.
-  Proof. iIntros "HT (?&?&?&?)". by iApply "HT". Qed.
+  Proof. iIntros "HT (?&?&?&?&?)". by iApply "HT". Qed.
   Global Instance simpl_padded_hyp_eq_layout_inst l β ty ly:
     SimplifyHypPlace l β (padded ty ly ly) (Some 0%N) :=
     λ T, i2p (simpl_padded_hyp_eq_layout l β ty ly T).
@@ -62,10 +73,12 @@ Section padded.
   Proof.
     revert select (LayoutEq _ _) => <-.
     iIntros "HT". iExists _. iFrame. iIntros "Hl". iDestruct (ty_aligned with "Hl") as %?.
-    do 2 iSplit => //. iFrame.
-    iExists []. rewrite heap_mapsto_own_state_nil. iPureIntro. split_and! => //.
-    - rewrite /has_layout_val/ly_offset/ly_size /=. lia.
-    - by apply: has_layout_ly_offset.
+    do 2 iSplit => //. iDestruct (movable_loc_in_bounds with "Hl") as "#Hb". iFrame "Hl Hb".
+    iExists []. rewrite heap_mapsto_own_state_nil.
+    iSplit. { iPureIntro. rewrite /has_layout_val/ly_offset/ly_size /=. lia. }
+    iSplit. { iPureIntro. by apply: has_layout_ly_offset. }
+    rewrite -{1}(Nat.add_0_r (ly_size _)) -loc_in_bounds_split.
+    by iDestruct "Hb" as "[_$]".
   Qed.
   Global Instance simpl_padded_goal_eq_layout_inst l ty ly `{!Movable ty} `{!LayoutEq (ty.(ty_layout)) ly}:
     SimplifyGoalPlace l Own (padded ty ly ly) (Some 0%N) :=
@@ -79,7 +92,7 @@ Section padded.
     (∀ l', typed_place K l' β1 ty (λ l2 ty2 β typ, T l2 ty2 β (λ t, padded (typ t) lyty ly))) -∗
     typed_place K l β1 (padded ty lyty ly) T.
   Proof.
-    iIntros "HP" (Φ) "(% & % & Hl & Hpad) HΦ" => /=.
+    iIntros "HP" (Φ) "(% & % & Hb & Hl & Hpad) HΦ" => /=.
     iApply ("HP" with "Hl"). iIntros (l2 β2 ty2 typ R) "Hl2 Hc".
     iApply ("HΦ" with "Hl2"). iIntros (ty') "Hl2".
     iMod ("Hc" with "Hl2") as "[$ $]". by iFrame.
@@ -95,7 +108,7 @@ Section padded.
     (∀ v, v◁ᵥty -∗ ⌜ty.(ty_layout) = lyty⌝ ∗ T) -∗
     subsume (l ◁ₗ padded ty lyty ly) (l ◁ₗ uninit ly) T.
   Proof.
-    iIntros "HT". iDestruct 1 as ([? ?] ?) "(Hl & Hr)".
+    iIntros "HT". iDestruct 1 as ([? ?] ?) "(Hb & Hl & Hr)".
     iDestruct (ty_deref with "Hl") as (v1) "[Hl Hv1]".
     iDestruct (ty_size_eq with "Hv1") as %Hlen1.
     iDestruct (ty_deref with "Hr") as (v2) "[Hr Hv2]".
@@ -115,6 +128,7 @@ Section padded.
     subsume (l ◁ₗ{β} uninit ly) (l ◁ₗ{β} padded (uninit lyty) lyty ly) T.
   Proof.
     iDestruct 1 as ([? ?]) "$". iIntros "Hl".
+    iDestruct (uninit_loc_in_bounds with "Hl") as "#$".
     iDestruct (split_uninit with "Hl") as "[Hl $]" => //. do 2 iSplit => //. by iDestruct "Hl" as (???) "?".
     iDestruct "Hl" as (v ??) "Hl". iExists _. iFrame. iSplit => //. iPureIntro.
     by apply: has_layout_loc_trans.
@@ -130,7 +144,7 @@ Section padded.
   Proof.
     iIntros "[% HT]" (Φ) "Hl".
     iDestruct (apply_subsume_place_true with "Hl []") as "Hl". iApply (subsume_uninit_padded _ _ _ sl) => //.
-    iApply "HT". iDestruct "Hl" as "[$ [$ [Hl $]]]". by rewrite uninit_struct_equiv.
+    iApply "HT". iDestruct "Hl" as "[$ [$ [$ [Hl $]]]]". by rewrite uninit_struct_equiv.
   Qed.
   Global Instance type_place_padded_uninit_struct_inst K l β sl n ly :
     TypedPlace (GetMemberPCtx sl n :: K) l β (uninit ly) :=
@@ -142,7 +156,7 @@ Section padded.
   Lemma padded_mono l β ty1 ty2 T ly1 ly2 lyty:
     ⌜ly1 = ly2⌝ ∗ subsume (l ◁ₗ{β} ty1) (l ◁ₗ{β} ty2) T -∗
     subsume (l ◁ₗ{β} padded ty1 lyty ly1) (l ◁ₗ{β} padded ty2 lyty ly2) T.
-  Proof. iIntros "[-> Hsub] ($&$&Hl&$)". by iApply "Hsub". Qed.
+  Proof. iIntros "[-> Hsub] ($&$&$&Hl&$)". by iApply "Hsub". Qed.
   Global Instance padded_mono_inst l β ty1 ty2 ly1 ly2 lyty:
     SubsumePlace l β (padded ty1 lyty ly1) (padded ty2 lyty ly2) :=
     λ T, i2p (padded_mono l β ty1 ty2 T ly1 ly2 lyty).
@@ -153,13 +167,14 @@ Section padded.
     l ◁ₗ{β} padded ty lyty ly1 -∗
       l ◁ₗ{β} padded ty lyty (ly_set_size ly1 n) ∗ (l +ₗ n) ◁ₗ{β} (uninit (ly_offset ly1 n)).
   Proof.
-    iIntros (? ?). iDestruct 1 as ([??]?) "($&Hl)".
+    iIntros (? ?). iDestruct 1 as ([??]?) "(#Hb&$&Hl)".
     (* iDestruct (split_uninit with "Hl") as "[? ?]". *)
     iDestruct "Hl" as (v Hv Hl) "Hmt".
     rewrite -[v](take_drop (n - lyty.(ly_size))%nat) heap_mapsto_own_state_app.
     iDestruct "Hmt" as "[Hmt1 Hmt2]". iSplitL "Hmt1".
-    - iSplit => //. iSplit; first by iPureIntro; apply: has_layout_loc_trans. iExists _. iFrame. iPureIntro.
-      split; last by apply has_layout_ly_offset.
+    - iSplit => //. iSplit; first by iPureIntro; apply: has_layout_loc_trans.
+      iSplit. { iApply loc_in_bounds_shorten; last done. rewrite /ly_size /= -/(ly_size _). lia. }
+      iExists _. iFrame. iPureIntro. split; last by apply has_layout_ly_offset.
       rewrite /has_layout_val take_length_le // Hv. rewrite {2}/ly_size/=. lia.
     - rewrite shift_loc_assoc take_length_le. 2: rewrite Hv {2}/ly_size/=; lia.
       have ->: (ly_size lyty + (n - ly_size lyty)%nat) = n by lia.
